cilc

coq/theories/cilc.v
@@ -664,10 +664,30 @@ Ltac fold_subst :=
   fold Subst_term;
   fold subst.
 
+Definition sing t := Cons t Nil.
+
+Fixpoint append (ls1 ls2 : terms) : terms :=
+  match ls1 with
+  | Nil => ls2
+  | Cons h ls1 => Cons h (append ls1 ls2)
+  end.
+
+Fixpoint rev (ls : terms) : terms :=
+  match ls with
+  | Nil => Nil
+  | Cons t ls => append (rev ls) (sing t)
+  end.
+
 Fixpoint spine (h : term) (ls : terms) : term :=
   match ls with
   | Nil => h
   | Cons m ls => spine (App h m) ls
+  end.
+
+Fixpoint spine' (h : term) (ls : terms) : term :=
+  match ls with
+  | Nil => h
+  | Cons m ls => App (spine' h ls) m
   end.
 
 Inductive iget : nat -> terms -> term -> Prop :=
@@ -687,7 +707,7 @@ Inductive step : term -> term -> Prop :=
 | step_AppR m n n' :
   step n n' ->
   step (App m n) (App m n')
-| step_beta m n :
+| step_Beta m n :
   step (App (Lam m) n) m.[n/]
 | step_ProdL A A' B s :
   step A A' ->
@@ -765,7 +785,7 @@ Inductive pstep : term -> term -> Prop :=
   pstep m m' ->
   pstep n n' ->
   pstep (App m n) (App m' n')
-| pstep_beta m m' n n' :
+| pstep_Beta m m' n n' :
   pstep m m' ->
   pstep n n' ->
   pstep (App (Lam m) n) (m'.[n'/])
@@ -792,6 +812,7 @@ Inductive pstep : term -> term -> Prop :=
   pstep' Fs Fs' ->
   pstep (Case m Q Fs) (Case m' Q' Fs')
 | pstep_CaseIota i m ms ms' Q Fs Fs' F F' :
+  iget i Fs F ->
   iget i Fs' F' ->
   pstep' ms ms' ->
   pstep' Fs Fs' ->
@@ -805,6 +826,7 @@ Inductive pstep : term -> term -> Prop :=
   pstep' Fs Fs' ->
   pstep (DCase m Q Fs) (DCase m' Q' Fs')
 | pstep_DCaseIota i m ms ms' Q Fs Fs' F F' :
+  iget i Fs F ->
   iget i Fs' F' ->
   pstep' ms ms' ->
   pstep' Fs Fs' ->
@@ -813,6 +835,9 @@ Inductive pstep : term -> term -> Prop :=
     (DCase (spine (Constr i m) ms) Q Fs)
     (spine F' ms')
 | pstep_Fix m m' :
+  pstep m m' ->
+  pstep (Fix m) (Fix m')
+| pstep_FixIota m m' :
   pstep m m' ->
   pstep (Fix m) (m'.[Fix m'/])
 
@@ -825,11 +850,129 @@ with pstep' : terms -> terms -> Prop :=
 
 Notation red := (star step).
 Notation red' := (star step').
-Notation conv := (conv step).
 Notation conv' := (conv step').
+Notation conv := (conv step).
 
 Definition sred sigma tau := 
   forall x : var, red (sigma x) (tau x).
+
+Lemma append_Nil ls : append ls Nil = ls.
+Proof. elim: ls=>//=. by move=> t ls ->. Qed.
+
+Lemma append_Cons m ls1 ls2 :
+  append (Cons m ls1) ls2 = Cons m (append ls1 ls2).
+Proof. by elim: ls1. Qed.
+
+Lemma append_assoc (xs ys zs : terms) :
+  append xs (append ys zs) = append (append xs ys) zs.
+Proof. elim: xs=> //=. by move=> t t0 ->. Qed.
+
+Lemma rev_append_distr (xs ys : terms) :
+  rev (append xs ys) = append (rev ys) (rev xs).
+Proof.
+  elim: xs ys=> //=.
+  move=> ys. by rewrite append_Nil.
+  move=> t ls ih ys. by rewrite ih append_assoc.
+Qed.
+
+Lemma rev_sing h ls :
+  rev (append ls (sing h)) = Cons h (rev ls).
+Proof. exact: rev_append_distr. Qed.
+
+Lemma rev_rev ls : rev (rev ls) = ls.
+Proof.
+  elim: ls=> //=.
+  move=> t ls e. by rewrite rev_sing e.
+Qed.
+
+Lemma append_sing_False h ls : ~Nil = append ls (sing h).
+Proof. elim: ls h=> //=. Qed.
+
+Lemma append_inj ls1 ls2 t1 t2 :
+  append ls1 (sing t1) = append ls2 (sing t2) ->
+    ls1 = ls2 /\ t1 = t2.
+Proof.
+  elim: ls1 ls2 t1 t2=> //=.
+  move=> ls1 t1 t2.
+    destruct ls1=> //= e.
+    by inv e.
+    rewrite /sing in e.
+    inv e.
+    by move: H1=> /append_sing_False.
+  move=> t ls1 ih ls2 t1 t2.
+    destruct ls2=> //= e.
+    rewrite /sing in e.
+    inv e.
+    exfalso.
+    apply: append_sing_False.
+    by rewrite <- H1.
+    inv e.
+    by move: H1=> /ih[->->].
+Qed.
+
+Lemma rev_inj ls1 ls2 : rev ls1 = rev ls2 -> ls1 = ls2.
+Proof.
+  elim: ls1 ls2=> //=.
+  move=> ls2. by destruct ls2=> //= /append_sing_False.
+  move=> t ls1 ih ls2.
+    destruct ls2=> //= e.
+    exfalso.
+    apply: append_sing_False.
+    by rewrite <- e.
+    move: e=> /append_inj[e1->].
+    by move: e1=> /ih ->.
+Qed.
+
+Lemma spine_append h xs ys :
+  spine h (append xs ys) = spine (spine h xs) ys.
+Proof. elim: xs ys h=> //=. Qed.
+
+Lemma spine_rev h m ls :
+  App (spine h (rev ls)) m = spine h (rev (Cons m ls)).
+Proof.
+  elim: ls h m=> //=.
+  move=> t ls ih h m.
+  rewrite spine_append=> //=.
+  rewrite spine_append=> //=.
+  by rewrite <- ih.
+Qed.
+
+Lemma spine_rev_spine' h ls :
+  spine h (rev ls) = spine' h ls.
+Proof.
+  elim: ls h=> //=.
+  move=> t t0 ih h.
+  rewrite <- ih.
+  by rewrite spine_rev.
+Qed.
+
+Lemma spine_spine'_rev h ls :
+  spine h ls = spine' h (rev ls).
+Proof.
+  have pf := spine_rev_spine' h (rev ls).
+  by rewrite rev_rev in pf.
+Qed.
+
+Lemma spine'_Constr i1 i2 h1 h2 ls1 ls2 :
+  spine' (Constr i1 h1) ls1 = spine' (Constr i2 h2) ls2 ->
+    i1 = i2 /\ h1 = h2 /\ ls1 = ls2.
+Proof.
+  elim: ls1 ls2 i1 i2 h1 h2=>//=.
+  move=> ls2 i1 i2 h1 h2.
+    destruct ls2=> //= e. by inv e.
+  move=> t ls1 ih ls2 t1 t2 h1 h2.
+    destruct ls2=> //= e.
+    inv e.
+    by move: H0=> /ih [->[->->]].
+Qed.
+
+Lemma spine_Constr i1 i2 h1 h2 ls1 ls2 :
+  spine (Constr i1 h1) ls1 = spine (Constr i2 h2) ls2 ->
+    i1 = i2 /\ h1 = h2 /\ ls1 = ls2.
+Proof.
+  rewrite! spine_spine'_rev=> /spine'_Constr[->[->e]].
+  by move: e=> /rev_inj->.
+Qed.
 
 Lemma spine_subst sigma h ls :
   (spine h ls).[sigma] = spine (h.[sigma]) (subst_terms sigma ls).
@@ -842,6 +985,15 @@ Proof.
     replace (App h.[sigma] a.[sigma]) with (App h a).[sigma]
       by autosubst.
     apply ih.
+Qed.
+
+Lemma iget_iget ls i m1 m2 :
+  iget i ls m1 -> iget i ls m2 -> m1 = m2.
+Proof.
+  move=> ig. elim: ig m2.
+  move=> m ls0 m2 ig. by inv ig.
+  move=> n m m' ls0 ig1 ih m2 ig2. inv ig2.
+    by move: H3=> /ih.
 Qed.
 
 Lemma iget_subst sigma i ls m :
@@ -861,7 +1013,7 @@ Proof.
     move=> m n sigma.
       replace (m.[n/].[sigma]) with (m.[up sigma].[n.[sigma]/])
         by autosubst.
-      apply step_beta.
+      apply step_Beta.
     move=> i m ms Q Fs F ig sigma; fold_subst.
       rewrite! spine_subst; asimpl.
       constructor.
@@ -873,7 +1025,7 @@ Proof.
     move=> m sigma.
       replace m.[Fix m/].[sigma] with m.[up sigma].[Fix m.[up sigma]/]
         by autosubst.
-      constructor.
+      constructor.    
   move=> st. elim: st sigma; asimpl; eauto using step'.
 Qed.
 
@@ -961,19 +1113,6 @@ Proof.
   apply: (star_hom Fix) A=> x y. exact: step_Fix.
 Qed.
 
-Lemma red_subst sigma m n :
-  red m n -> red m.[sigma] n.[sigma].
-Proof.
-  move=> rd. elim: rd sigma=> /={n}.
-  move=> sigma //.
-  move=> y z rd ih st sigma.
-    have rd1 := ih sigma.
-    apply: star_trans.
-    apply: rd1.
-    move: st=> /(step_subst sigma) rd2.
-    by apply: star1.
-Qed.
-
 Lemma red'_h h1 h2 ls :
   red h1 h2 -> red' (Cons h1 ls) (Cons h2 ls).
 Proof.
@@ -992,6 +1131,53 @@ Proof.
   apply: star_trans.
     by apply: ih.
     by apply: star1; constructor.
+Qed.
+
+Lemma red'_Nil ls : red' Nil ls -> ls = Nil.
+Proof. 
+  elim=> //.
+  move=> y z _ -> st. by inv st.
+Qed.
+
+Lemma red'_Cons m ls l : 
+  red' (Cons m ls) l -> 
+    exists m' ls', l = Cons m' ls' /\ red m m' /\ red' ls ls'.
+Proof.
+  elim=> //.
+  by exists m; exists ls=> //.
+  move=> y z rd [m0 [ls0 [-> [rd1 rd2]]]] st. inv st.
+    exists m'; exists ls0; split=> //.
+      split. apply: starSE. exact: rd1. exact: H2. exact: rd2.
+    exists m0; exists ls'; split=> //.
+      split. exact: rd1. apply: starSE. exact: rd2. exact: H2.
+Qed.
+
+Lemma red_spine h h' ls ls' :
+  red h h' -> red' ls ls' -> red (spine h ls) (spine h' ls').
+Proof.
+  elim: ls ls' h h'.
+  move=> ls' h h' rd /red'_Nil -> //.
+  move=> t t0 ih ls' h h' rd rd'=> //=.
+  apply: (star_trans (spine (App h' t) t0)).  
+    apply: ih=> //.
+    exact: red_App.
+  move: rd'=> /red'_Cons [m [ls [-> [rd1 rd2]]]] //=.
+    apply: ih.
+    exact: red_App.
+    exact: rd2.
+Qed.
+
+Lemma red_subst sigma m n :
+  red m n -> red m.[sigma] n.[sigma].
+Proof.
+  move=> rd. elim: rd sigma=> /={n}.
+  move=> sigma //.
+  move=> y z rd ih st sigma.
+    have rd1 := ih sigma.
+    apply: star_trans.
+    apply: rd1.
+    move: st=> /(step_subst sigma) rd2.
+    by apply: star1.
 Qed.
 
 Lemma sred_up sigma tau : 
@@ -1020,3 +1206,515 @@ Proof.
       apply: red'_h; exact: red_compat.
       apply: red'_ls; exact: ih.
 Qed.
+
+Definition sconv (sigma tau : var -> term) := 
+  forall x, conv (sigma x) (tau x).
+
+Lemma conv_Lam m1 m2 : conv m1 m2 -> conv (Lam m1) (Lam m2).
+Proof. apply: conv_hom=> x y. exact: step_Lam. Qed.
+
+Lemma conv_Prod A1 A2 s B1 B2 :
+  conv A1 A2 -> conv B1 B2 -> conv (Prod A1 B1 s) (Prod A2 B2 s).
+Proof.
+  move=> A B.
+  apply: (conv_trans (Prod A2 B1 s)).
+  apply: (conv_hom ((Prod^~ B1)^~ s)) A => x y ps.
+    by constructor.
+  apply: (conv_hom ((Prod A2)^~ s)) B => x y ps.
+    by constructor.
+Qed.
+
+Lemma conv_Lolli A1 A2 s B1 B2 :
+  conv A1 A2 -> conv B1 B2 -> conv (Lolli A1 B1 s) (Lolli A2 B2 s).
+Proof.
+  move=> A B.
+  apply: (conv_trans (Lolli A2 B1 s)).
+  apply: (conv_hom ((Lolli^~ B1)^~ s)) A => x y ps.
+    by constructor.
+  apply: (conv_hom ((Lolli A2)^~ s)) B => x y ps.
+    by constructor.
+Qed.
+
+Lemma conv_App m1 m2 n1 n2 :
+  conv m1 m2 -> conv n1 n2 -> conv (App m1 n1) (App m2 n2).
+Proof.
+  move=> A B.
+  apply: (conv_trans (App m2 n1)).
+  apply: (conv_hom (App^~ n1)) A=> x y ps.
+    by constructor.
+  apply: conv_hom B=> x y ps.
+    by constructor.
+Qed.
+
+Lemma conv_Ind A1 A2 s Cs1 Cs2 :
+  conv A1 A2 -> conv' Cs1 Cs2 -> conv (Ind A1 s Cs1) (Ind A2 s Cs2).
+Proof.
+  move=> A B. 
+  apply: (conv_trans (Ind A2 s Cs1)).
+  apply: (conv_hom ((Ind^~ s)^~ Cs1)) A=> x y. exact: step_IndA.
+  elim: B=> //.
+    move=> y z cv' cv st.
+    apply: (conv_trans (Ind A2 s y)).
+      by apply: cv.
+      by apply: conv1; eauto using step.
+    move=> y z cv' cv st.
+    apply: (conv_trans (Ind A2 s y)).
+      by apply: cv.
+      by apply: conv1i; eauto using step.
+Qed.
+
+Lemma conv_Constr i m1 m2 :
+  conv m1 m2 -> conv (Constr i m1) (Constr i m2).
+Proof.
+  move=> A.
+  apply: (conv_hom (Constr i)) A => x y. exact: step_Constr.
+Qed.
+
+Lemma conv_Case m1 m2 Q1 Q2 Fs1 Fs2 :
+  conv m1 m2 -> conv Q1 Q2 -> conv' Fs1 Fs2 -> conv (Case m1 Q1 Fs1) (Case m2 Q2 Fs2).
+Proof.
+  move=> A B C. 
+  apply: (conv_trans (Case m2 Q1 Fs1)).
+  apply: (conv_hom ((Case^~ Q1)^~ Fs1)) A=> x y. exact: step_CaseM.
+  apply: (conv_trans (Case m2 Q2 Fs1)).
+  apply: (conv_hom ((Case m2)^~ Fs1)) B=> x y. exact: step_CaseQ.
+  elim: C=> //.
+    move=> y z cv' cv st.
+    apply: conv_trans.
+      by apply: cv.
+      by apply: conv1; eauto using step.
+    move=> y z cv' cv st.
+    apply: conv_trans.
+      by apply: cv.
+      by apply: conv1i; eauto using step.
+Qed.
+
+Lemma conv_DCase m1 m2 Q1 Q2 Fs1 Fs2 :
+  conv m1 m2 -> conv Q1 Q2 -> conv' Fs1 Fs2 -> conv (DCase m1 Q1 Fs1) (DCase m2 Q2 Fs2).
+Proof.
+  move=> A B C. 
+  apply: (conv_trans (DCase m2 Q1 Fs1)).
+  apply: (conv_hom ((DCase^~ Q1)^~ Fs1)) A=> x y. exact: step_DCaseM.
+  apply: (conv_trans (DCase m2 Q2 Fs1)).
+  apply: (conv_hom ((DCase m2)^~ Fs1)) B=> x y. exact: step_DCaseQ.
+  elim: C=> //.
+    move=> y z rd' rd st.
+    apply: conv_trans.
+      by apply: rd.
+      by apply: conv1; eauto using step.
+    move=> y z rd' rd st.
+    apply: conv_trans.
+      by apply: rd.
+      by apply: conv1i; eauto using step.
+Qed.
+
+Lemma conv_Fix m1 m2 :
+  conv m1 m2 -> conv (Fix m1) (Fix m2).
+Proof.
+  move=> A.
+  apply: (conv_hom Fix) A=> x y. exact: step_Fix.
+Qed.
+
+Lemma conv'_h h1 h2 ls :
+  conv h1 h2 -> conv' (Cons h1 ls) (Cons h2 ls).
+Proof.
+  move=> cv. elim: cv ls=> //.
+  move=> y z cv ih st ls.
+    apply: conv_trans.
+      by apply: ih.
+      by apply: conv1; constructor.
+  move=> y z rd ih st ls.
+    apply: conv_trans.
+      by apply: ih.
+      by apply: conv1i; constructor.
+Qed.
+
+Lemma conv'_ls h ls ls' :
+  conv' ls ls' -> conv' (Cons h ls) (Cons h ls').
+Proof.
+  move=> cv. elim: cv h=> //.
+  move=> y z cv ih st h.
+    apply: conv_trans.
+      by apply: ih.
+      by apply: conv1; constructor.
+  move=> y z cv ih st h.
+    apply: conv_trans.
+      by apply: ih.
+      by apply: conv1i; constructor.
+Qed.
+
+Lemma conv_subst sigma m n :
+  conv m n -> conv m.[sigma] n.[sigma].
+Proof.
+  move=> cv. elim: cv sigma=> /={n}.
+  move=> sigma //.
+  move=> y z rd ih st sigma.
+    have cv1 := ih sigma.
+    apply: conv_trans.
+    apply: cv1.
+    move: st=> /(step_subst sigma) rd2.
+    by apply: conv1.
+  move=> y z rd ih st sigma.
+    have cv1 := ih sigma.
+    apply: conv_trans.
+    apply: cv1.
+    move: st=> /(step_subst sigma) rd2.
+    by apply: conv1i.
+Qed.
+
+Lemma sconv_up sigma tau : 
+  sconv sigma tau -> sconv (up sigma) (up tau).
+Proof. 
+  move=> A [|n] //=; asimpl. 
+  apply: conv_subst. 
+  exact: A. 
+Qed.
+
+Hint Resolve 
+  conv_App conv_Lam conv_Prod conv_Lolli 
+  conv_Ind conv_Constr conv_Case conv_DCase conv_Fix
+  conv_subst sconv_up 
+: conv_congr.
+
+Lemma conv_compat sigma tau s : 
+  sconv sigma tau -> conv s.[sigma] s.[tau]
+with conv_compat' sigma tau ls :
+  sconv sigma tau -> conv' (subst_terms sigma ls) (subst_terms tau ls).
+Proof. 
+  elim: s sigma tau=> {conv_compat}; asimpl; eauto 6 with conv_congr.
+  elim: ls sigma tau=> {conv_compat'}; asimpl; eauto 6 with conv_congr.
+    move=> t t0 ih sigma tau sr.
+    apply: conv_trans.
+      apply: conv'_h; exact: conv_compat.
+      apply: conv'_ls; exact: ih.
+Qed.
+
+Lemma conv_Beta s t1 t2 : conv t1 t2 -> conv s.[t1/] s.[t2/].
+Proof. move=> c. by apply: conv_compat => -[]. Qed.
+
+Lemma pstep_refl s : pstep s s
+with pstep_refl' ls : pstep' ls ls.
+Proof. 
+  elim: s=> /={pstep_refl}; eauto using pstep.
+  elim: ls=> /={pstep_refl'}; eauto using pstep'.
+Qed.
+
+Lemma step_pstep m m' : step m m' -> pstep m m'
+with step_pstep' ls ls' : step' ls ls' -> pstep' ls ls'.
+Proof with eauto using pstep, pstep', pstep_refl, pstep_refl'.
+  elim {step_pstep}...
+  elim {step_pstep'}...
+Qed.
+
+Lemma pstep_red m m' : pstep m m' -> red m m'
+with pstep_red' ls ls' : pstep' ls ls' -> red' ls ls'.
+Proof.
+  elim=> {m m' pstep_red} //=; eauto with red_congr.
+    move=> m m' n n' p1 r1 p2 r2.
+      apply: starES.
+      by econstructor.
+      apply: (star_trans (m'.[n.:Var])). exact: red_subst.
+      by apply: red_compat => -[|].
+    move=> i m ms ms' Q Fs Fs' F F' ig ig' p1 p2 p3 r.
+      have ih1 := pstep_red' _ _ p1=> {p1}.
+      have ih2 := pstep_red' _ _ p2=> {p2}.
+      apply: star_trans.
+      apply: red_Case.
+      apply: red_spine.
+      exact: starR.
+      exact: ih1.
+      exact: starR.
+      exact: ih2.
+      apply: star1.
+      by constructor.
+    move=> i m ms ms' Q Fs Fs' F F' ig ig' p1 p2 p3 r.
+      have ih1 := pstep_red' _ _ p1=> {p1}.
+      have ih2 := pstep_red' _ _ p2=> {p2}.
+      apply: star_trans.
+      apply: red_DCase.
+      apply: red_spine.
+      exact: starR.
+      exact: ih1.
+      exact: starR.
+      exact: ih2.
+      apply: star1.
+      by constructor.
+    move=> m m' p r.
+      apply: star_trans.
+      apply: red_Fix.
+      exact: r.
+      apply: star1.
+      by constructor.
+  elim=> {ls ls' pstep_red'} //=.
+    move=> m m' ls ls' p1 p2 r.
+    apply: (star_trans (Cons m' ls)).
+      apply: red'_h. exact: pstep_red.
+      exact: red'_ls.
+Qed.
+
+Lemma pstep_subst sigma m m' :
+  pstep m m' -> pstep m.[sigma] m'.[sigma]
+with pstep_subst' sigma ls ls' :
+  pstep' ls ls' -> pstep' (subst_terms sigma ls) (subst_terms sigma ls').
+Proof with eauto using pstep, pstep', pstep_refl, pstep_refl'.
+  move=> p. elim: p sigma => {m m' pstep_subst}...
+  move=> m m' n n' p1 ih1 p2 ih2 sigma; asimpl.
+    have h1 := (ih1 (up sigma))=> {ih1}.
+    have h2 := (ih2 sigma)=> {ih2}.
+    have h3 := pstep_Beta (h1 Ids_term Rename_term) h2.
+    by asimpl in h3.
+  move=> i m ms ms' Q Fs Fs' F F' ig ig' p1 p2 p3 ih sigma=> //=; fold_subst.
+    rewrite! spine_subst; fold_subst.
+    apply: pstep_CaseIota; eauto.
+    apply: iget_subst. exact ig.
+    apply: iget_subst. exact ig'.
+  move=> i m ms ms' Q Fs Fs' F F' ig ig' p1 p2 p3 ih sigma=> //=; fold_subst.
+    rewrite! spine_subst; fold_subst.
+    apply: pstep_DCaseIota; eauto.
+    apply: iget_subst. exact ig.
+    apply: iget_subst. exact ig'.
+  move=> m m' p ih sigma; asimpl.
+    replace m'.[Fix m'.[up sigma] .: sigma]
+      with (m'.[up sigma]).[Fix m'.[up sigma]/]
+      by autosubst.
+    exact: pstep_FixIota.
+  elim=> {ls ls' pstep_subst'}...
+Qed.
+
+Definition psstep (sigma tau : var -> term) := 
+  forall x, pstep (sigma x) (tau x).
+
+Lemma psstep_refl sigma : psstep sigma sigma.
+Proof with eauto using pstep_refl.
+  unfold psstep.
+  induction x...
+Qed.
+
+Lemma psstep_up sigma tau :
+  psstep sigma tau -> psstep (up sigma) (up tau).
+Proof with eauto using pstep, pstep_refl.
+  move=> A [|n] //=. asimpl... asimpl; apply: pstep_subst. exact: A.
+Qed.
+
+Lemma pstep_compat sigma tau m m' :
+  pstep m m' -> psstep sigma tau -> pstep m.[sigma] m'.[tau]
+with pstep_compat' sigma tau ls ls' :
+  pstep' ls ls' -> 
+    psstep sigma tau -> pstep' (subst_terms sigma ls) (subst_terms tau ls').
+Proof with eauto 6 using pstep, pstep', psstep_up.
+  move=> p. 
+  elim: p sigma tau => {m m' pstep_compat}...
+    move=> m m' n n' p1 ih1 p2 ih2 sigma tau ps1; asimpl.
+      have ps2 := psstep_up ps1.
+      have h1 := ih1 _ _ ps2.
+      have h2 := ih2 _ _ ps1.
+      have h3 := pstep_Beta h1 h2.
+      by asimpl in h3.
+    move=> i m ms ms' Q Fs Fs' F F' ig ig' p1 p2 p3 ih sigma tau ps=> //=; fold_subst.
+      rewrite! spine_subst; fold_subst.
+      apply: pstep_CaseIota.
+      apply: iget_subst. exact: ig.
+      apply: iget_subst. exact: ig'.
+      exact: pstep_compat'.
+      exact: pstep_compat'.
+      exact: ih.
+    move=> i m ms ms' Q Fs Fs' F F' ig ig' p1 p2 p3 ih sigma tau ps=> //=; fold_subst.
+      rewrite! spine_subst; fold_subst.
+      apply: pstep_DCaseIota.
+      apply: iget_subst. exact: ig.
+      apply: iget_subst. exact: ig'.
+      exact: pstep_compat'.
+      exact: pstep_compat'.
+      exact: ih.
+    move=> m m' p ih sigma tau ps; asimpl.
+      replace m'.[Fix m'.[up tau] .: tau]
+        with (m'.[up tau]).[Fix m'.[up tau]/]
+        by autosubst.
+      constructor.
+      apply: ih.
+      exact: psstep_up.
+  elim=> {ls ls' pstep_compat'}...
+Qed.
+
+Lemma psstep_compat sigma tau m1 m2 :
+  psstep sigma tau -> pstep m1 m2 -> psstep (m1 .: sigma) (m2 .: tau).
+Proof. move=> A B [|n] //=. Qed.
+
+Lemma pstep_subst_term m n n' :
+  pstep n n' -> pstep m.[n/] m.[n'/].
+Proof with eauto using pstep, pstep', pstep_refl, pstep_refl'.
+  move=> p.
+  apply: pstep_compat...
+  apply: psstep_compat...
+  exact: psstep_refl.
+Qed.
+
+Lemma pstep_compat_Beta m m' n n' :
+  pstep m m' -> pstep n n' -> pstep m.[n/] m'.[n'/].
+Proof with eauto using psstep_refl, psstep_compat.
+  move=> p1 p2.
+  apply: pstep_compat...
+Qed.
+
+Lemma pstep'_iget1 ls ls' i m :
+  pstep' ls ls' -> iget i ls m -> exists m', iget i ls' m' /\ pstep m m'.
+Proof with eauto using iget.
+  move=> p.
+  elim: p m i => {ls ls'}.
+  move=> m i ig. inv ig.
+  move=> m m' ls ls' p1 p2 ih m0 i ig. inv ig.
+    exists m'...
+    move: H3=> /ih [m'0 [ig p]].
+    exists m'0...
+Qed.
+
+Lemma pstep'_iget2 ls ls' i m' :
+  pstep' ls ls' -> iget i ls' m' -> exists m, iget i ls m /\ pstep m m'.
+Proof with eauto using iget.
+  move=> p.
+  elim: p m' i => {ls ls'}.
+  move=> m' i ig. inv ig.
+  move=> m m' ls ls' p1 p2 ih m0 i ig. inv ig.
+    exists m...
+    move: H3=> /ih[m1 [ig p]].
+    exists m1...
+Qed.
+
+Lemma pstep_spine h h' ls ls' :
+  pstep h h' -> pstep' ls ls' -> pstep (spine h ls) (spine h' ls').
+Proof.
+  elim: ls ls' h h'.
+  move=> ls' h h' p1 p2. inv p2=> //=.
+  move=> t t0 ih ls h h' p p'. inv p'=> //=.
+  apply: ih=> //.
+  exact: pstep_App.
+Qed.
+
+Lemma pstep_spine_inv h ls m :
+  pstep (spine h ls) m -> (~ exists m, h = Lam m) -> 
+    exists h' ls', m = spine h' ls' /\ pstep h h' /\ pstep' ls ls'.
+Proof with eauto using pstep, pstep', pstep_refl, pstep_refl'.
+  elim: ls h m.
+  move=> h m //= p nx.
+  exists m; exists Nil...
+  move=> t t0 ih h m //= p nx.
+  move: p=> /ih p.
+  have pf : ~ (exists m, App h t = Lam m).
+    apply: all_not_not_ex=> n.
+    have pf := classic (App h t = Lam n).
+    inv pf=> //.
+  move: pf=> /p [h' [ls' [-> [p1 p2]]]].
+  inv p1.
+  exists m'; exists (Cons n' ls')...
+  exfalso.
+  apply: nx.
+  by exists m0.
+Qed.
+
+Lemma pstep_diamond m m1 m2 :
+  pstep m m1 -> pstep m m2 -> exists m', pstep m1 m' /\ pstep m2 m'
+with pstep_diamond' ls ls1 ls2 :
+  pstep' ls ls1 -> pstep' ls ls2 -> exists ls', pstep' ls1 ls' /\ pstep' ls2 ls'.
+Proof with eauto 6 using pstep, pstep', pstep_compat_Beta, pstep_spine.
+  move=> p. 
+  elim: p m2=> {m m1 pstep_diamond}.
+    move=> x m2 p. inv p. exists (Var x)...
+    move=> srt l m2 p. inv p. exists (Sort srt l)...
+    move=> n n' p1 ih m2 p2. inv p2.
+      move: H0=> /ih [m' [p2 p3]].
+      exists (Lam m')...
+    move=> m m' n n' p1 ih1 p2 ih2 m2 p3. inv p3.
+      move: H1=> /ih1 [m'1 [p3 p4]].
+      move: H3=> /ih2 [m'2 [p5 p6]].
+      exists (App m'1 m'2)...
+      inv p1.
+      have h : pstep (Lam m0) (Lam m'0).
+        by constructor.
+      move: h=> /ih1 [m' [p3 p4]].
+      move: H3=> /ih2 [m'1 [p5 p6]].
+      inv p3; inv p4.
+      exists (n'2.[m'1/])... 
+    move=> m m' n n' p1 ih1 p2 ih2 m2 p3. inv p3.
+      inv H1.
+      move: H0=> /ih1 [m'0 [p3 p4]].
+      move: H3=> /ih2 [m'1 [p5 p6]].
+      exists (m'0.[m'1/])...
+      move: H1=> /ih1 [m'1 [p3 p4]].
+      move: H3=> /ih2 [m'2 [p5 p6]].
+      exists (m'1.[m'2/])...
+    move=> A A' s B B' p1 ih1 p2 ih2 m2 p3. inv p3.
+      move: H3=> /ih1 [m' [p3 p4]].
+      move: H4=> /ih2 [m'0 [p5 p6]].
+      exists (Prod m' m'0 s)...
+    move=> A A' s B B' p1 ih1 p2 ih2 m2 p3. inv p3.
+      move: H3=> /ih1 [m' [p3 p4]].
+      move: H4=> /ih2 [m'0 [p5 p6]].
+      exists (Lolli  m' m'0 s)...
+    move=> A A' s Cs Cs' p1 ih p2 m2 p3. inv p3.
+      move: H3=> /ih [m' [p3 p4]].
+      move: (pstep_diamond' _ _ _ p2 H4)=> [ls' [p5 p6]].
+      exists (Ind m' s ls')...
+    move=> i m m' p1 ih m2 p2. inv p2.
+      move: H2=> /ih [m'1 [p2 p3]].
+      exists (Constr i m'1)...
+    move=> m m' Q Q' Fs Fs' p1 ih1 p2 ih2 p3 m2 p4. inv p4.
+      move: H2=> /ih1 [m'1 [p4 p5]].
+      move: H4=> /ih2 [m'2 [p6 p7]].
+      move: (pstep_diamond' _ _ _ p3 H5)=> [ls' [p8 p9]].
+      exists (Case m'1 m'2 ls')...
+      have pf :  ~(exists m : term, Constr i m0 = Lam m).
+        move=> [m e] //=.
+      move: p1=> /pstep_spine_inv p1.
+      move: pf=> /p1 [h' [ls'0 [-> [p4 p6]]]]. inv p4. 
+      move: (pstep_diamond' _ _ _ p6 H4)=> [ls' [p7 p8]].
+      move: (pstep_diamond' _ _ _ p3 H6)=> [ls'1 [p9 p10]].
+      move: (pstep'_iget1 p10 H3)=> [F1 [ig1 p11]].
+      move: (pstep'_iget2 p9 ig1)=> [F2 [ig2 p12]].
+      exists (spine F1 ls')...
+    move=> i m ms ms' Q Fs Fs' F F' ig ig' p1 p2 p3 ih m2 p4. inv p4.
+      have pf :  ~(exists m0 : term, Constr i m = Lam m0).
+        move=> [m0 e] //=.
+      move: H2=> /pstep_spine_inv H2.
+      move: pf=> /H2 [h' [ls' [-> [p4 p5]]]]. inv p4.
+      move: (pstep_diamond' _ _ _ p2 H5)=> [ls'0 [p6 p7]].
+      move: (pstep_diamond' _ _ _ p1 p5)=> [ls'1 [p8 p9]].
+      move: (pstep'_iget1 p6 ig')=> [m'1 [ig1 p10]].
+      move: (pstep'_iget2 p7 ig1)=> [m'2 [ig2 p11]].
+      exists (spine m'1 ls'1)...
+      move: H=> /spine_Constr[e1 [e2 e3]]; subst.
+      move: (pstep_diamond' _ _ _ p1 H4)=> [ls'0 [p6 p7]].
+      move: (pstep'_iget1 H6 ig)=> [F1 [ig1 p8]].
+      move: (iget_iget ig1 H3)=> e; subst.
+      move: p8=> /ih[F2 [p9 p10]].
+      exists (spine F2 ls'0)...
+    move=> m m' Q Q' Fs Fs' p1 ih1 p2 ih2 p3 m2 p4. inv p4.
+      move: H2=> /ih1 [m'1 [p4 p5]].
+      move: H4=> /ih2 [m'2 [p6 p7]].
+      move: (pstep_diamond' _ _ _ p3 H5)=> [ls' [p8 p9]].
+      exists (DCase m'1 m'2 ls')...
+      have pf :  ~(exists m : term, Constr i m0 = Lam m).
+        move=> [m e] //=.
+      move: p1=> /pstep_spine_inv p1.
+      move: pf=> /p1 [h' [ls'0 [-> [p4 p6]]]]. inv p4. 
+      move: (pstep_diamond' _ _ _ p6 H4)=> [ls' [p7 p8]].
+      move: (pstep_diamond' _ _ _ p3 H6)=> [ls'1 [p9 p10]].
+      move: (pstep'_iget1 p10 H3)=> [F1 [ig1 p11]].
+      move: (pstep'_iget2 p9 ig1)=> [F2 [ig2 p12]].
+      exists (spine F1 ls')...
+    move=> i m ms ms' Q Fs Fs' F F' ig ig' p1 p2 p3 ih m2 p4. inv p4.
+      have pf :  ~(exists m0 : term, Constr i m = Lam m0).
+        move=> [m0 e] //=.
+      move: H2=> /pstep_spine_inv H2.
+      move: pf=> /H2 [h' [ls' [-> [p4 p5]]]]. inv p4.
+      move: (pstep_diamond' _ _ _ p2 H5)=> [ls'0 [p6 p7]].
+      move: (pstep_diamond' _ _ _ p1 p5)=> [ls'1 [p8 p9]].
+      move: (pstep'_iget1 p6 ig')=> [m'1 [ig1 p10]].
+      move: (pstep'_iget2 p7 ig1)=> [m'2 [ig2 p11]].
+      exists (spine m'1 ls'1)...
+      move: H=> /spine_Constr[e1 [e2 e3]]; subst.
+      move: (pstep_diamond' _ _ _ p1 H4)=> [ls'0 [p6 p7]].
+      move: (pstep'_iget1 H6 ig)=> [F1 [ig1 p8]].
+      move: (iget_iget ig1 H3)=> e; subst.
+      move: p8=> /ih[F2 [p9 p10]].
+      exists (spine F2 ls'0)...
+      
